LeanHoG/Invariant/HamiltonianPath/Tactic.lean
@@ -4,9 +4,11 @@ import LeanHoG.LoadGraph
 import LeanHoG.Invariant.HamiltonianPath.SatEncoding
 import LeanHoG.Tactic.Options
 
+import LeanSAT
+
 namespace LeanHoG
 
-open Lean Widget Elab Command Term Meta Qq
+open Lean Widget Elab Command Term Meta Qq LeanSAT Model Tactic
 
 -- def loadHamiltonianPathData (filePath : System.FilePath) : IO HamiltonianPathData := do
 --   let fileContent ← IO.FS.readFile filePath
@@ -16,7 +18,6 @@ open Lean Widget Elab Command Term Meta Qq
 
 syntax (name := computeHamiltonianPath) "#compute_hamiltonian_path " ident : command
 
-open ProofWidgets in
 @[command_elab computeHamiltonianPath]
 unsafe def computeHamiltonianPathImpl : CommandElab
   | `(#compute_hamiltonian_path $g ) => liftTermElabM do
@@ -46,6 +47,70 @@ unsafe def computeHamiltonianPathImpl : CommandElab
     }
     Lean.Meta.addInstance hamiltonianPathName .scoped 42
     logInfo "found Hamiltonian path"
+
+  | _ => throwUnsupportedSyntax
+
+syntax (name := showNoHamiltonianPath) "#show_no_hamiltonian_path " ident : command
+
+unsafe def showNoHamiltonianPathAux (graphName : Name) (graph : Q(Graph)) : TermElabM (Name × Q(Prop)) := do
+    let G ← evalExpr' Graph ``Graph graph
+    let enc := (hamiltonianPathCNF G).val
+    -- let cadicalExe := "/home/jure/source-control/cadical/build/cadical"
+    -- let cake_lprExr := "/home/jure/source-control/cake_lpr/cake_lpr"
+    -- let solver := LeanSAT.Solver.Impl.CakeLpr cadicalExe #["--no-binary"] cake_lprExr
+    let solver : LeanSAT.Solver IO := (LeanSAT.Solver.Impl.DimacsCommand "/home/jure/source-control/cadical/build/cadical")
+    let cnf := Encode.EncCNF.toICnf enc
+    let res ← solver.solve cnf
+    match res with
+    | .sat _sol =>
+      throwError "graph has Hamiltonian path"
+    | .unsat =>
+      -- The formula is UNSAT, add an axiom saying so
+      let declName : Name := .str graphName "noHamiltonianPathCertificateExists"
+      let type : Q(Prop) := q(¬ (∃ (τ : PropAssignment (Var (Graph.vertexSize $graph))), τ |> hamiltonianPathConstraints $graph))
+      let decl := Declaration.axiomDecl {
+        name        := declName,
+        levelParams := [],
+        type        := type,
+        isUnsafe    := false
+      }
+      trace[Elab.axiom] "{declName} : {type}"
+      Term.ensureNoUnassignedMVars decl
+      addDecl decl
+      return (declName, type)
+    | .error => throwError "SAT solver exited with error"
+
+/-- `#show_no_hamiltonian_path G` runs a SAT solver on the encoding of the Hamiltonian path problem
+    on the graph `G` and if the SAT solver says the problem is unsat it runs the produced proof
+    through a verified proof checker cake_lpr. If the checker agrees with the proof, we add an axiom
+    saying there exists no satisfying assignmment for the encoding.
+-/
+@[command_elab showNoHamiltonianPath]
+unsafe def showNoHamiltonianPathImpl : CommandElab
+  | `(#show_no_hamiltonian_path $g ) => liftTermElabM do
+    let graphName := g.getId
+    let graph ← Qq.elabTermEnsuringTypeQ g q(Graph)
+    let (declName, type) ← showNoHamiltonianPathAux graphName graph
+    logInfo m!"added axiom {declName} : {type}"
+
+  | _ => throwUnsupportedSyntax
+
+syntax (name := showNoHamiltonianPathTactic) "show_no_hamiltonian_path " ident : tactic
+
+@[tactic showNoHamiltonianPathTactic]
+unsafe def showNoHamiltonianPathTacticImpl : Tactic
+  | `(tactic|show_no_hamiltonian_path $g) =>
+    withMainContext do
+      let graphName := g.getId
+      let graph ← Qq.elabTermEnsuringTypeQ g q(Graph)
+      let (declName, type) ← showNoHamiltonianPathAux graphName graph
+      let noExistsCert ← Tactic.elabTermEnsuringType (mkIdent declName) type
+      let noExistsHamPath ← mkAppM ``LeanHoG.no_assignment_implies_no_hamiltonian_path' #[noExistsCert]
+      let noExistsType := q(¬ ∃ (u v : Graph.vertex $graph) (p : Path $graph u v), p.isHamiltonian)
+      liftMetaTactic fun mvarId => do
+        let mvarIdNew ← mvarId.assert .anonymous noExistsType noExistsHamPath
+        let (_, mvarIdNew) ← mvarIdNew.intro1P
+        return [mvarIdNew]
 
   | _ => throwUnsupportedSyntax
 
